\begin{thm}
    Dado un grupo $G = \{X, \cdot\}$, si para todo $a,b \in G$ se cumple que $(a\cdot b)^2 = a^2 \cdot b^2$, entonces $G$ es abeliano
    \begin{equation}
        \forall a,b \in G: (a\cdot b)^2 = a^2 \cdot b^2 \implies \forall a,b \in G: a \cdot b = b \cdot a
    \end{equation}
\end{thm}

\begin{proof}
    \begin{equation}
        \begin{split}
        & (a \cdot b)^2 = a^2 \cdot b^2 \implies abab = aabb \iff a^{-1}(abab) = a^{-1}(aabb) \iff\\
        & bab = abb \iff (bab)b^{-1} = (abb)b^{-1} \iff ba = ab  
        \end{split}
    \end{equation}
\end{proof}
