\begin{lem}
    Dado un grupo $G = \{X, \cdot\}$, para cada pareja $a,b \in G$ se cumple que $(a\cdot b)^{-1}=b^{-1}a^{-1}$
    \label{lem:inverso}
\end{lem}

\begin{proof}
    \begin{equation}
        \begin{split}
            & (a \cdot b)^{-1} (a \cdot b) = e \iff (a\cdot b)^{-1}(a\cdot b)\cdot b^{-1} = e \cdot b^{-1} \iff\\
            & (a\cdot b)^{-1}a = b^{-1} \iff (a\cdot b)^{-1}a\cdot a^{-1} = b^{-1}a^{-1} \iff\\
            & (a\cdot b)^{-1} = b^{-1} a^{-1}
        \end{split}
    \end{equation}
\end{proof}

\begin{thm}
    Dado un grupo $G = \{X, \cdot\}$, para cada pareja $a,b \in G$ el orden de $ab$ es el mismo que el de $ba$
    \begin{equation}
        \forall a,b \in G: (a\cdot b)^{k} = e \iff (b \cdot a)^{k} = e  
    \end{equation}
\end{thm}

\begin{proof}
    \begin{equation}
        \begin{split}
        & (ab)^{k} = ab\cdot ab\cdots ab = a \cdot (ba \cdots ba) \cdot b = a \cdot (ba)^{k-1} \cdot b = e \iff\\
        & a^{-1}\cdot a\cdot (ba)^{k-1}\cdot b = a^{-1} \iff (ba)^{k-1}\cdot b = a^{-1} \iff\\
        & (ba)^{k-1}\cdot b \cdot b^{-1}  = a^{-1}b^{-1} \iff (ba)^{k-1} = a^{-1}b^{-1} \annoterel{\text{lema} \ref{lem:inverso}}{=} (ba)^{-1} \iff\\
        & (ba)^{k-1}(ba) = (ba)^{-1}(ba) \iff (ba)^{k} = e   
        \end{split}
    \end{equation}
\end{proof}
